basis/RatProgScript.sml
@@ -1,44 +1,12 @@
 open preamble ml_translatorLib ml_translatorTheory ml_progLib
-    mlvectorTheory mlintProgTheory basisFunctionsLib
-open simpLib realTheory realLib RealArith
-open ml_translatorTheory ml_translatorLib std_preludeTheory;
-open gcdTheory;
+     mlvectorTheory IntProgTheory basisFunctionsLib
+     realTheory realLib RealArith gcdTheory
 
-val _ = new_theory"mlratProg"
+val _ = new_theory"RatProg"
 
-val _ = translation_extends "mlintProg";
+val _ = translation_extends "IntProg";
 
 val _ = ml_prog_update (open_module "Rat");
-
-val real_of_int_def = Define `
-  real_of_int (i:int) = if i < 0 then - & (Num (-i)) else & (Num i):real`;
-
-val real_of_int_num = store_thm("real_of_int_num[simp]",
-  ``real_of_int (& n) = &n``,
-  rewrite_tac[real_of_int_def]
-  \\ Cases_on `(&n):int`
-  \\ fs []);
-
-val real_of_int_add = store_thm("real_of_int_add[simp]",
-  ``real_of_int (m + n) = real_of_int m + real_of_int n``,
-  Cases_on `m` \\ Cases_on `n` \\ fs [real_of_int_def] \\ rw []
-  \\ fs [integerTheory.INT_ADD_CALCULATE]
-  \\ rw [] \\ fs [] \\ fs [GSYM NOT_LESS,realTheory.add_ints]);
-
-val real_of_int_neg = store_thm("real_of_int_neg[simp]",
-  ``real_of_int (-m) = -real_of_int m``,
-  Cases_on `m` \\ fs [real_of_int_def]);
-
-val real_of_int_sub = store_thm("real_of_int_sub[simp]",
-  ``real_of_int (m - n) = real_of_int m - real_of_int n``,
-  fs [integerTheory.int_sub,realTheory.real_sub]);
-
-val real_of_int_mul = store_thm("real_of_int_mul[simp]",
-  ``real_of_int (m * n) = real_of_int m * real_of_int n``,
-  Cases_on `m` \\ Cases_on `n` \\ fs [real_of_int_def] \\ rw []
-  \\ fs [integerTheory.INT_MUL_CALCULATE]);
-
-(* -- *)
 
 val REAL_TYPE_def = Define `
   REAL_TYPE (r:real) =
